code/poly1305/Hacl.Impl.Poly1305.fst
@@ -28,10 +28,16 @@ unfold
 let op_String_Access #a #len = LSeq.index #a #len
 
 inline_for_extraction noextract
-let get_acc #s (ctx:poly1305_ctx s) = sub ctx 0ul (nlimb s)
+let get_acc #s (ctx:poly1305_ctx s) : Stack (felem s)
+  (requires fun h -> live h ctx)
+  (ensures  fun h0 acc h1 -> h0 == h1 /\ live h1 acc /\ acc == gsub ctx 0ul (nlimb s))
+  = sub ctx 0ul (nlimb s)
 
 inline_for_extraction noextract
-let get_precomp_r #s (ctx:poly1305_ctx s) = sub ctx (nlimb s) (precomplen s)
+let get_precomp_r #s (ctx:poly1305_ctx s) : Stack (precomp_r s)
+  (requires fun h -> live h ctx)
+  (ensures  fun h0 pre h1 -> h0 == h1 /\ live h1 pre /\ pre == gsub ctx (nlimb s) (precomplen s))
+  = sub ctx (nlimb s) (precomplen s)
 
 let as_get_acc #s h ctx = (feval h (gsub ctx 0ul (nlimb s))).[0]
 let as_get_r #s h ctx = (feval h (gsub ctx (nlimb s) (nlimb s))).[0]
